pcuic/theories/PCUICConversionInversion.v
@@ -1,9 +1,11 @@
 From Equations Require Import Equations.
 From MetaCoq.PCUIC Require Import PCUICAst.
 From MetaCoq.PCUIC Require Import PCUICAstUtils.
+From MetaCoq.PCUIC Require Import PCUICContextConversion.
 From MetaCoq.PCUIC Require Import PCUICCumulativity.
 From MetaCoq.PCUIC Require Import PCUICCumulProp.
 From MetaCoq.PCUIC Require Import PCUICEquality.
+From MetaCoq.PCUIC Require Import PCUICLiftSubst.
 From MetaCoq.PCUIC Require Import PCUICNormal.
 From MetaCoq.PCUIC Require Import PCUICReduction.
 From MetaCoq.PCUIC Require Import PCUICTyping.
@@ -29,16 +31,6 @@ Section fixed.
     eq_term_upto_univ_napp Σ (eq_universe Σ) (conv_pb_rel leq Σ) napp.
   
   Notation eq_termp leq := (eq_termp_napp leq 0).
-  
-  Lemma eq_termp_mkApps_inv leq v args v' args' :
-    isApp v = false ->
-    isApp v' = false ->
-    eq_termp leq (mkApps v args) (mkApps v' args') ->
-    eq_termp_napp leq #|args| v v' × All2 (fun x y => eq_term Σ Σ x y) args args'.
-  Proof.
-    intros noapp1 noapp2 eq.
-    now apply eq_term_upto_univ_mkApps_inv in eq as (?&?).
-  Qed.
   
   Definition isIndConstructApp (t : term) : bool :=
     match (decompose_app t).1 with
@@ -84,17 +76,42 @@ Section fixed.
     - now rewrite !isIndConstructApp_mkApps.
     - now rewrite !isIndConstructApp_mkApps.
   Qed.
-
-  Lemma whne_red_isIndConstructApp Γ t t' :
-    whne RedFlags.default Σ Γ t ->
+  
+  Lemma whnf_red1_isIndConstructApp Γ t t' :
+    whnf RedFlags.default Σ Γ t ->
+    red1 Σ Γ t t' ->
+    isIndConstructApp t' = isIndConstructApp t.
+  Proof.
+    intros wh r.
+    depelim wh.
+    - eapply whne_red1_isIndConstructApp; eauto.
+    - depelim r; solve_discr.
+    - depelim r; auto; solve_discr.
+    - depelim r; auto; solve_discr.
+    - apply red1_mkApps_tConstruct_inv in r as (?&->&?).
+      now rewrite !isIndConstructApp_mkApps.
+    - apply red1_mkApps_tInd_inv in r as (?&->&?).
+      now rewrite !isIndConstructApp_mkApps.
+    - apply red1_mkApps_tFix_inv in r.
+      2: { destruct unfold_fix as [(?&?)|]; [|easy].
+           now unfold is_constructor; rewrite H. }
+      now destruct r as [[(?&->&o)|(?&->&o)]|(?&->&o)];
+        rewrite !isIndConstructApp_mkApps.
+    - apply red1_mkApps_tCoFix_inv in r.
+      now destruct r as [[(?&->&o)|(?&->&o)]|(?&->&o)];
+        rewrite !isIndConstructApp_mkApps.
+  Qed.
+  
+  Lemma whnf_red_isIndConstructApp Γ t t' :
+    whnf RedFlags.default Σ Γ t ->
     red Σ Γ t t' ->
     isIndConstructApp t' = isIndConstructApp t.
   Proof.
     intros wh r.
     induction r in wh |- * using red_rect_n1.
     - easy.
-    - apply whne_red1_isIndConstructApp in X as ->; eauto.
-      eapply whne_pres; eauto.
+    - apply whnf_red1_isIndConstructApp in X as ->; eauto.
+      eapply whnf_pres; eauto.
   Qed.
 
   Lemma conv_cum_alt leq Γ t t' :
@@ -114,6 +131,16 @@ Section fixed.
     cbn.
     now apply PCUICCumulProp.eq_term_upto_univ_napp_leq.
   Qed.
+  
+  Lemma eq_termp_mkApps_inv leq v args v' args' :
+    isApp v = false ->
+    isApp v' = false ->
+    eq_termp leq (mkApps v args) (mkApps v' args') ->
+    eq_termp_napp leq #|args| v v' × All2 (fun x y => eq_term Σ Σ x y) args args'.
+  Proof.
+    intros noapp1 noapp2 eq.
+    now apply eq_term_upto_univ_mkApps_inv in eq as (?&?).
+  Qed.
 
   Lemma conv_cum_mkApps_inv leq Γ hd args hd' args' :
     conv_cum leq Σ Γ (mkApps hd args) (mkApps hd' args') ->
@@ -129,26 +156,37 @@ Section fixed.
     | tConstruct _ _ _ => False
     | _ => True
     end ->
-    whne RedFlags.default Σ Γ hd ->
-    whne RedFlags.default Σ Γ hd' ->
+    whnf RedFlags.default Σ Γ (mkApps hd args) ->
+    whnf RedFlags.default Σ Γ (mkApps hd' args') ->
     ∥conv_cum leq Σ Γ hd hd' × All2 (conv Σ Γ) args args'∥.
   Proof.
     intros conv shape shape' wh wh'.
     apply conv_cum_alt in conv as [(?&?&(r1&r2)&e)].
-    eapply whne_red_from_mkApps in r1; auto; [|now destruct hd].
-    destruct r1 as [(?&?&->&?&?)].
-    eapply whne_red_from_mkApps in r2; auto; [|now destruct hd'].
-    destruct r2 as [(?&?&->&?&?)].
-    apply eq_termp_mkApps_inv in e as (?&?).
-    2-3: erewrite whne_red_isApp; [| |now eauto]; eauto; try now destruct hd, hd'.
+    apply whnf_red_from_mkApps in r1 as [(?&?&->&?&?)]; auto.
+    apply whnf_red_from_mkApps in r2 as [(?&?&->&?&?)]; auto.
+    assert (isApp x1 = false).
+    { erewrite whnf_red_isApp.
+      3: eauto.
+      1: now destruct hd.
+      apply whnf_mkApps_inv in wh; auto.
+      now destruct hd. }
+    assert (isApp x = false).
+    { erewrite whnf_red_isApp.
+      3: eauto.
+      1: now destruct hd'.
+      apply whnf_mkApps_inv in wh'; auto.
+      now destruct hd'. }
+    apply eq_termp_mkApps_inv in e as (?&?); auto.
     constructor.
     split.
     - apply conv_cum_alt.
       constructor.
       exists x1, x.
-      split; eauto.
+      split; [split|]; eauto with pcuic.
       eapply eq_term_upto_univ_napp_nonind; eauto.
-      erewrite whne_red_isIndConstructApp; [| |now eauto]; eauto.
+      erewrite whnf_red_isIndConstructApp; [| |now eauto].
+      1: now destruct hd.
+      apply whnf_mkApps_inv in wh; auto.
       now destruct hd.
     - clear -a1 a a0.
       induction a1 in args, args', x2, a, x3, a0, a1 |- *; depelim a; depelim a0; [now constructor|].
@@ -189,7 +227,118 @@ Section fixed.
     + now apply IHa1.
   Qed.
   
-  (* TODO: Remove to a place that actually should be depending on typing *)
+  Lemma fix_context_change_decl_types Γ mfix mfix' :
+    #|mfix| = #|mfix'| ->
+    context_relation (fun _ _ => change_decl_type) (Γ,,, fix_context mfix) (Γ,,, fix_context mfix').
+  Proof.
+    intros len.
+    apply context_relation_app_inv.
+    - now rewrite !fix_context_length.
+    - apply context_relation_refl.
+      intros.
+      destruct x.
+      destruct decl_body; constructor.
+    - unfold fix_context, mapi.
+      generalize 0 at 2 4.
+      induction mfix in mfix', len |- *; intros n.
+      + destruct mfix'; [|cbn in *; discriminate len].
+        constructor.
+      + destruct mfix'; cbn in *; [discriminate len|].
+        apply context_relation_app_inv.
+        * now rewrite !List.rev_length, !mapi_rec_length.
+        * constructor; [constructor|].
+          constructor.
+        * apply IHmfix; lia.
+  Qed.
+  
+  Lemma red_tFix_inv Γ mfix idx t :
+    red Σ Γ (tFix mfix idx) t ->
+    ∑ mfix',
+     t = tFix mfix' idx ×
+     All2 (fun d d' => dname d = dname d' × rarg d = rarg d' ×
+                       red Σ Γ (dtype d) (dtype d') ×
+                       red Σ (Γ,,, fix_context mfix) (dbody d) (dbody d'))
+          mfix mfix'.
+  Proof.
+    intros r.
+    remember (tFix mfix idx) eqn:fromeq.
+    revert mfix fromeq.
+    induction r using red_rect_n1; intros mfix ->.
+    - eexists _; split; [reflexivity|].
+      apply All2_same.
+      eauto.
+    - specialize (IHr _ eq_refl) as (?&->&all).
+      depelim X.
+      + exfalso.
+        destruct args using List.rev_ind; [|rewrite <- mkApps_nested in H; discriminate H].
+        unfold is_constructor in e0.
+        rewrite nth_error_nil in e0; congruence.
+      + match type of all with
+        | All2 ?P _ _ => eapply OnOne2_All2 with (Q := P) in o
+        end; eauto.
+        2: intros ? ? (?&[= -> -> ->]); eauto.
+        eexists _; split; [reflexivity|].
+        eapply All2_trans; eauto.
+        intros ? ? ? (?&?&?&?) (?&?&?&?); eauto.
+        do 2 (split; [easy|]).
+        split; [etransitivity; eauto|].
+        etransitivity; eauto.
+      + match type of all with
+        | All2 ?P _ _ => eapply OnOne2_All2 with (Q := P) in o
+        end; eauto.
+        2: { intros ? ? (?&[= -> -> ->]); eauto.
+             do 2 (split; [easy|]).
+             split; [etransitivity; eauto|].
+             eapply context_change_decl_types_red; eauto.
+             apply fix_context_change_decl_types.
+             apply All2_length in all.
+             easy. }
+        eexists _; split; [reflexivity|].
+        eapply All2_trans; eauto.
+        intros ? ? ? (?&?&?&?) (?&?&?&?); eauto.
+        do 2 (split; [easy|]).
+        split; [etransitivity; eauto|].
+        etransitivity; eauto.
+  Qed.
+  
+  Lemma conv_cum_tFix_inv leq Γ mfix idx mfix' idx' :
+    conv_cum leq Σ Γ (tFix mfix idx) (tFix mfix' idx') ->
+    ∥idx = idx' ×
+     All2 (fun d d' => rarg d = rarg d' ×
+                       Σ;;; Γ |- dtype d = dtype d' ×
+                       Σ;;; Γ,,, fix_context mfix |- dbody d = dbody d')
+          mfix mfix'∥.
+  Proof.
+    intros conv.
+    apply conv_cum_alt in conv as [(?&?&(r1&r2)&?)].
+    apply red_tFix_inv in r1 as (?&->&?).
+    apply red_tFix_inv in r2 as (?&->&?).
+    depelim e.
+    constructor.
+    split; [easy|].
+    clear -a a0 a1.
+    cut (#|mfix| = #|mfix'|);
+      [|now apply All2_length in a; apply All2_length in a0; apply All2_length in a1].
+    revert a a0 a1.
+    generalize mfix at 1 3 4.
+    generalize mfix' at 1 3.
+    intros ctx_fix ctx_fix'.
+    intros all1 all2 all len_eq.
+    induction all in mfix, mfix', x1, x, all1, all2, all |- *;
+      depelim all1; depelim all2; [constructor|].
+    constructor; [|now auto].
+    destruct p as (?&?&?&?), p0 as (?&?&?&?), r as ((?&?)&?).
+    split; [congruence|].
+    split; [now apply conv_alt_red; exists (dtype x), (dtype y)|].
+    apply conv_alt_red.
+    exists (dbody x), (dbody y).
+    split; [|easy].
+    split; [easy|].
+    eapply context_change_decl_types_red; eauto.
+    eapply fix_context_change_decl_types; eauto.
+  Qed.
+  
+  (* TODO: Move to a place that actually should be depending on typing *)
   Lemma conv_cum_red_inv leq Γ t1 t2 t1' t2' :
     conv_cum leq Σ Γ t1 t2 ->
     red Σ Γ t1 t1' ->
